ulib/LowStar.PrefixFreezableBuffer.fst
@@ -1,0 +1,150 @@
+(*
+   Copyright 2008-2018 Microsoft Research
+
+   Licensed under the Apache License, Version 2.0 (the "License");
+   you may not use this file except in compliance with the License.
+   You may obtain a copy of the License at
+
+       http://www.apache.org/licenses/LICENSE-2.0
+
+   Unless required by applicable law or agreed to in writing, software
+   distributed under the License is distributed on an "AS IS" BASIS,
+   WITHOUT WARRANTIES OR CONDITIONS OF ANY KIND, either express or implied.
+   See the License for the specific language governing permissions and
+   limitations under the License.
+*)
+
+module LowStar.PrefixFreezableBuffer
+
+open FStar.HyperStack.ST
+
+include LowStar.Monotonic.Buffer
+
+module P = FStar.Preorder
+module G = FStar.Ghost
+
+module U8 = FStar.UInt8
+module U32 = FStar.UInt32
+module Seq = FStar.Seq
+
+module HS = FStar.HyperStack
+module ST = FStar.HyperStack.ST
+
+
+(*
+ * Implementation for LowStar.PrefixfreezableBuffer
+ *)
+
+#set-options "--max_fuel 0 --max_ifuel 0"
+
+/// Read a sequence of bytes as a nat in the little-endian order
+///
+/// Going forward it will come from LowStar.Endianness
+
+assume val le_to_n (s:Seq.seq u8) : Tot nat
+assume val le_to_n_zeros (s:Seq.seq u8)
+  : Lemma
+    (requires
+      Seq.length s >= 4 /\
+      (forall (i:nat). i < Seq.length s ==> Seq.index s i == 0uy))
+    (ensures le_to_n (Seq.slice s 0 4) == 0)
+
+let frozen_until s = le_to_n (Seq.slice s 0 4)
+
+let prefix_freezable_preorder = pre
+
+let prefix_freezable_preorder_elim _ _ = ()
+
+
+/// A store32_le function that stores a u32 in a bytes buffer in le format
+///
+/// Going forward it will come from LowStar.Endianness
+
+assume private val store32_le
+  (b:mbuffer u8 prefix_freezable_preorder prefix_freezable_preorder)
+  (i:u32)
+  : Stack
+    unit
+    (requires fun h ->
+      live h b /\
+      4 <= length b /\
+      frozen_until (as_seq h b) <= U32.v i /\ U32.v i <= length b)
+    (ensures  fun h0 _ h1 ->
+      live h1 b /\
+       modifies (loc_buffer b) h0 h1 /\
+       frozen_until (as_seq h1 b) == U32.v i /\
+       (forall (k:nat).{:pattern (Seq.index (as_seq h1 b) k)}
+          (k >= 4 /\ k < length b) ==> Seq.index (as_seq h1 b) k == Seq.index (as_seq h0 b) k))
+
+private let update_frozen_until_alloc
+  (b:mbuffer u8 prefix_freezable_preorder prefix_freezable_preorder)
+  : Stack
+    unit
+    (requires fun h ->
+      live h b /\
+      length b >= 4 /\
+      frozen_until (as_seq h b) == 0)
+    (ensures  fun h0 _ h1 ->
+      live h1 b /\
+      modifies (loc_buffer b) h0 h1 /\
+      frozen_until (as_seq h1 b) == 4 /\
+      witnessed b (frozen_until_at_least 4))
+  = store32_le b 4ul;
+    witness_p b (frozen_until_at_least 4)
+
+let gcmalloc r len =
+  let h0 = ST.get () in
+  
+  let b = mgcmalloc #_ #prefix_freezable_preorder r 0uy (U32.add len 4ul) in
+
+  let h = ST.get () in le_to_n_zeros (as_seq h b);
+
+  assert (fresh_loc (loc_buffer b) h0 h);  //TODO: necessary for firing modifies_remove_new_locs lemma?
+  update_frozen_until_alloc b;
+  b
+
+let malloc r len =
+  let h0 = ST.get () in
+  
+  let b = mmalloc #_ #prefix_freezable_preorder r 0uy (U32.add len 4ul) in
+
+  let h = ST.get () in le_to_n_zeros (as_seq h b);
+
+  assert (fresh_loc (loc_buffer b) h0 h);  //TODO: necessary for firing modifies_remove_new_locs lemma?
+  update_frozen_until_alloc b;
+  b
+
+let alloca len =
+  let h0 = ST.get () in
+  
+  let b = malloca #_ #prefix_freezable_preorder 0uy (U32.add len 4ul) in
+
+  let h = ST.get () in le_to_n_zeros (as_seq h b);
+
+  assert (fresh_loc (loc_buffer b) h0 h);  //TODO: necessary for firing modifies_remove_new_locs lemma?
+  update_frozen_until_alloc b;
+  b
+
+let upd b i v =
+  recall_p b (frozen_until_at_least 4);
+  upd b i v
+
+let freeze b i =
+  recall_p b (frozen_until_at_least 4);
+  store32_le b i;
+  witness_p b (frozen_until_at_least (U32.v i))
+
+let witness_slice b i j snap =
+  witness_p b (slice_is i j snap)
+
+let recall_slice b i j snap =
+  recall_p b (slice_is i j snap)
+
+let witness_frozen_until b n =
+  witness_p b (frozen_until_at_least n)
+
+let recall_frozen_until b n =
+  recall_p b (frozen_until_at_least n)
+
+let recall_frozen_until_default b =
+  recall_p b (frozen_until_at_least 4)
